Done

NatDoubleInduction.thy
@@ -4,7 +4,8 @@ hide_const Suc
 datatype nat = Zero | Suc nat
 
 
-text "Example exlpains a proof for a cutom induction rule"
+section "How to define custom induction rules"
+subsection "Example for cutom induction rules"
 lemma nat_induct: "\<lbrakk> P Zero; \<And>n. P n \<Longrightarrow> P (Suc n) \<rbrakk> \<Longrightarrow> P n"
   apply(rule nat.induct)
   apply(assumption)
@@ -12,40 +13,114 @@ lemma nat_induct: "\<lbrakk> P Zero; \<And>n. P n \<Longrightarrow> P (Suc n) \<
   done
 
 
-text "Lemma to proof the double induction rule"
-lemma nat_induct_N_0: "\<lbrakk> P Zero Zero; \<And>m n. P m n \<Longrightarrow> P (Suc m) n; \<And>m n. P m n \<Longrightarrow> P m (Suc n) \<rbrakk> \<Longrightarrow> P m Zero"
-  apply(erule_tac n=m in nat_induct)
-  apply(assumption)
-  done
-
-
-text "Double induction rule for \<nat> \<times> \<nat>"
-theorem nat_induct_M_N: "\<lbrakk> P Zero Zero; \<And>m n. P m n \<Longrightarrow> P (Suc m) n; \<And>m n. P m n \<Longrightarrow> P m (Suc n) \<rbrakk> \<Longrightarrow> P m n"
-  apply(rule nat_induct)
-  apply(erule nat_induct_N_0)
-  apply(assumption)
-  apply(assumption)
-  apply(assumption)
-  done
-
-
 fun nat_eq :: "nat \<Rightarrow> nat \<Rightarrow> bool" where
-  "nat_eq Zero Zero = True" |
-  "nat_eq (Suc n) Zero = False" |
-  "nat_eq Zero (Suc m) = False" |
-  "nat_eq (Suc n) (Suc m) = nat_eq n m"
+  nat_eq_ZeroZero: "nat_eq Zero Zero = True" |
+  nat_eq_SucZero:  "nat_eq (Suc n) Zero = False" |
+  nat_eq_ZeroSuc:  "nat_eq Zero (Suc m) = False" |
+  nat_eq_SucSuc:   "nat_eq (Suc n) (Suc m) = nat_eq n m"
 
 
-text "Example using the induction rule that implemented by me"
+text "Single-induction example using the custom induction rule"
 lemma nat_eq_refl: "nat_eq n n"
   apply(rule nat_induct)
-  apply(subst nat_eq.simps)
+  apply(subst nat_eq_ZeroZero)
   apply(rule TrueI)
-  apply(subst nat_eq.simps)
+  apply(subst nat_eq_SucSuc)
   apply(assumption)
   done
 
 
-(* TODO: Example using nat_induct_M_N *)
+lemma nat_eq_sym[rule_format]: "\<forall>n. nat_eq m n \<longleftrightarrow> nat_eq n m"
+  apply(rule nat_induct)
+  apply(rule allI)
+  apply(rule_tac y=n in nat.exhaust)
+  apply(erule ssubst)
+  apply(subst (1 2) nat_eq_ZeroZero)
+  apply(rule refl)
+  apply(erule ssubst)
+  apply(subst nat_eq_SucZero)
+  apply(subst nat_eq_ZeroSuc)
+  apply(rule refl)
+  apply(rule allI)
+  apply(rule_tac y=na in nat.exhaust)
+  apply(erule ssubst)
+  apply(subst nat_eq_SucZero)
+  apply(subst nat_eq_ZeroSuc)
+  apply(rule refl)
+  apply(erule ssubst)
+  apply(subst (1 2) nat_eq_SucSuc)
+  apply(drule_tac x=x2 in spec)
+  apply(assumption)
+  done
 
+
+fun nat_plus :: "nat \<Rightarrow> nat \<Rightarrow> nat" where
+  nat_plus_ZeroFree: "nat_plus Zero n = n" |
+  nat_plus_SucFree:  "nat_plus (Suc m) n = nat_plus m (Suc n)"
+
+
+lemma nat_plus_FreeSuc[rule_format]: "\<forall>n. nat_plus m (Suc n) = Suc (nat_plus m n)"
+  apply(rule_tac n=m in nat_induct)
+  apply(subst (1 2) nat_plus_ZeroFree)
+  apply(rule allI)
+  apply(rule refl)
+
+  apply(simp only: nat_plus_SucFree)
+  apply(rule allI)
+  apply(subst nat.simps(1))
+  apply(subst nat.simps(1))
+  apply(rule refl)
+  done
+
+
+subsection "Double-induction example using the custom induction rule"
+lemma "nat_eq (nat_plus m n) (nat_plus n m)"
+  apply(rule_tac n=m in nat_induct)
+  apply(rule_tac n=n in nat_induct)
+  apply(unfold nat_plus_ZeroFree nat_eq_ZeroZero)
+  apply(rule TrueI)
+
+  apply(rule_tac y=n in nat.exhaust)
+  apply(clarify)
+  apply(unfold nat_plus_SucFree nat_plus_ZeroFree nat_eq_SucSuc nat_eq_ZeroZero)
+  apply(rule TrueI)
+
+  apply(clarify)
+  apply(unfold nat_plus_SucFree nat_plus_ZeroFree nat_plus_FreeSuc nat_eq_SucSuc)
+  apply(assumption)
+  apply(assumption)
+  done
+
+
+section "How to define double-induction rules"
+subsection "Lemmas to proof the double induction rule"
+lemma nat_induct_N_M: "\<lbrakk> P Zero Zero; \<And>m n. P m n \<Longrightarrow> P (Suc m) n; \<And>m n. P m n \<Longrightarrow> P m (Suc n) \<rbrakk> \<Longrightarrow> P m n"
+  apply(rule_tac n=m in nat_induct)
+  apply(rule_tac n=n in nat_induct)
+  apply(assumption)
+
+  apply(drule_tac P="\<lambda>m. (\<And>n. P m n \<Longrightarrow> P m (Suc n))"  and x="Zero" in meta_spec)
+  apply(drule_tac P="\<lambda>n. (P Zero n \<Longrightarrow> P Zero (Suc n))"  and x="n" in meta_spec)
+  apply(drule meta_mp)
+  apply(assumption)
+  apply(assumption)
+
+  apply(drule_tac P="\<lambda>m. (\<And>n. P m n \<Longrightarrow> P (Suc m) n)" and x="na" in meta_spec)
+  apply(drule_tac P="\<lambda>n. (P na n \<Longrightarrow> P (Suc na) n)" and x="n" in meta_spec)
+  apply(drule meta_mp)
+  apply(assumption)
+  apply(assumption)
+  done
+
+
+subsection "Proof using the custom double-induction rule"
+lemma "nat_eq (nat_plus m n) (nat_plus n m)"
+  apply(rule_tac n=n and m=m in nat_induct_N_M)
+  apply(unfold nat_plus_ZeroFree)
+  apply(subst nat_eq_ZeroZero)
+  apply(rule TrueI)
+  apply(unfold nat_plus_SucFree nat_plus_FreeSuc nat_eq_SucSuc)
+  apply(assumption)
+  apply(assumption)
+  done
 end
